Solved `ticket_lock.v`

exercises/ticket_lock.v
@@ -61,8 +61,8 @@ Definition release : val :=
   specifications to figure out exactly what needs to be proven.
 *)
 
-Definition RA : cmra
-  (* := insert your definition here *). Admitted.
+Definition RA : cmra :=
+  authR (prodUR (optionUR (exclR natO)) (gset_disjR nat)).
 
 Section proofs.
 Context `{!heapGS Σ, !inG Σ RA}.
@@ -73,8 +73,8 @@ Let N := nroot .@ "ticket_lock".
   specific ticket. As such, we first define a predicate [locked_by]
   which states that the lock is locked by ticket [o].
 *)
-Definition locked_by (γ : gname) (o : nat) : iProp Σ
-  (* := insert your definition here *). Admitted.
+Definition locked_by (γ : gname) (o : nat) : iProp Σ :=
+  own γ (◯ (Excl' o, GSet ∅)).
 
 (** The lock is locked when it has been locked by some ticket. *)
 Definition locked (γ : gname) : iProp Σ :=
@@ -82,19 +82,24 @@ Definition locked (γ : gname) : iProp Σ :=
 
 Lemma locked_excl γ : locked γ -∗ locked γ -∗ False.
 Proof.
-  (* exercise *)
-Admitted.
+  iIntros "[%o1 Hγ1] [%o2 Hγ2]".
+  iCombine "Hγ1 Hγ2" gives "%H".
+  rewrite auth_frag_valid /= pair_valid /= in H.
+  by destruct H.
+Qed.
 
 (**
   We will also have a predicate signifying that ticket [x] has been
   _issued_. A thread will need to have been issued ticket [x] in order
   to wait for the first counter to become [x].
 *)
-Definition issued (γ : gname) (x : nat) : iProp Σ
-  (* := insert your definition here *). Admitted.
+Definition issued (γ : gname) (x : nat) : iProp Σ :=
+  own γ (◯ (ε, GSet {[x]})).
 
-Definition lock_inv (γ : gname) (lo ln : loc) (P : iProp Σ) : iProp Σ
-  (* := insert your definition here *). Admitted.
+Definition lock_inv (γ : gname) (lo ln : loc) (P : iProp Σ) : iProp Σ :=
+  ∃ o n : nat, lo ↦ #o ∗ ln ↦ #n ∗ 
+  own γ (● (Excl' o, GSet (set_seq 0 n))) ∗
+  ((locked_by γ o ∗ P) ∨ issued γ o).
 
 Definition is_lock (γ : gname) (l : val) (P : iProp Σ) : iProp Σ :=
   ∃ lo ln : loc, ⌜l = (#lo, #ln)%V⌝ ∗ inv N (lock_inv γ lo ln P).
@@ -105,27 +110,136 @@ Definition is_lock (γ : gname) (l : val) (P : iProp Σ) : iProp Σ :=
 Lemma mk_lock_spec P :
   {{{ P }}} mk_lock #() {{{ γ l, RET l; is_lock γ l P }}}.
 Proof.
-  (* exercise *)
-Admitted.
+  iIntros "%Φ P HΦ".
+  rewrite /mk_lock; wp_pures.
+  wp_alloc ln as "Hln".
+  wp_alloc lo as "Hlo".
+  wp_pures.
+  iMod (own_alloc (● (Excl' 0, GSet ∅) ⋅ ◯ (Excl' 0, GSet ∅))) as "(%γ & Hγ & Ho)";
+    first by apply auth_both_valid_discrete.
+  iApply ("HΦ" $! γ).
+  iExists lo, ln.
+  iSplitR; first done.
+  iMod (inv_alloc with "[P Hln Hlo Hγ Ho]") as "#I"; last by iFrame "#".
+  iExists 0, 0.
+  iFrame.
+  iLeft.
+  iFrame.
+Qed.
 
 Lemma wait_spec γ l P x :
   {{{ is_lock γ l P ∗ issued γ x }}}
     wait #x l
   {{{ RET #(); locked γ ∗ P }}}.
 Proof.
-  (* exercise *)
-Admitted.
+  iIntros "%Φ [(%lo & %ln & -> & #I) Hx] HΦ".
+  iLöb as "IH".
+  wp_rec.
+  wp_pures.
+  wp_bind (! _)%E.
+  iInv "I" as "(%o & %n & Hlo & Hln & Hγ)".
+  wp_load.
+  destruct (decide (#o = #x)).
+  - injection e as e.
+    apply (inj Z.of_nat) in e; subst x.
+    iDestruct "Hγ" as "[Hγ [[Hexcl P]|Ho]]".
+    + iSplitL "Hlo Hln Hγ Hx"; first by iFrame.
+      iModIntro; wp_pures.
+      rewrite bool_decide_eq_true_2; last done.
+      wp_pures.
+      iApply "HΦ".
+      by iFrame.
+    + iCombine "Hx Ho" gives "%H".
+      rewrite auth_frag_valid /= pair_valid /= in H.
+      destruct H as [_ H].
+      apply gset_disj_valid_op in H.
+      by rewrite disjoint_singleton_l not_elem_of_singleton in H.
+  - iSplitL "Hlo Hln Hγ"; first by iFrame.
+    iModIntro; wp_pures.
+    rewrite bool_decide_eq_false_2; last done.
+    wp_pures.
+    by iApply ("IH" with "Hx").
+Qed.
 
 Lemma acquire_spec γ l P :
   {{{ is_lock γ l P }}} acquire l {{{ RET #(); locked γ ∗ P }}}.
 Proof.
-  (* exercise *)
-Admitted.
+  iIntros "%Φ (%lo & %ln & -> & #I) HΦ".
+  iLöb as "IH".
+  wp_rec; wp_pures.
+  wp_bind (! _)%E.
+  iInv "I" as "(%o & %n & Hlo & Hln & Hγ)".
+  wp_load.
+  iSplitL "Hlo Hln Hγ"; first by iFrame.
+  clear o.
+  iModIntro; wp_pures.
+  wp_bind (CmpXchg _ _ _).
+  iInv "I" as "(%o & %n' & Hlo & Hln & Hγ)".
+  destruct (decide (#n = #n')).
+  - injection e as e.
+    apply (inj Z.of_nat) in e; subst n'.
+    wp_cmpxchg_suc.
+    assert (#(n + 1) = #(S n)) as ->.
+    { rewrite -(Nat2Z.inj_add _ 1). 
+      by (replace (S n) with (n + 1) by lia). }
+    iDestruct "Hγ" as "[Hγ Hγ']".
+    iMod (own_update _ _ (● (Excl' o, GSet (set_seq 0 (S n))) ⋅ ◯ (ε, GSet {[n]})) with "Hγ") as "[Hγ Hn]".
+    { apply auth_update_alloc, prod_local_update_2.
+      assert (GSet {[n]} ≡ GSet {[n]} ⋅ ε) as -> by rewrite right_id //.
+      assert (GSet (set_seq 0 (S n)) ≡ GSet {[n]} ⋅ GSet (set_seq 0 n)) as ->.
+      { rewrite set_seq_S_end_union_L gset_disj_union.
+        - done.
+        - replace n with (0 + n) at 1 by lia. 
+          apply set_seq_S_end_disjoint. }
+      apply gset_disj_alloc_op_local_update.
+      replace n with (0 + n) at 1 by lia. 
+      apply set_seq_S_end_disjoint. }
+    rewrite {2}/lock_inv.
+    iSplitL "Hlo Hln Hγ Hγ'"; first by iFrame.
+    iModIntro; wp_pures.
+    wp_apply (wait_spec with "[$Hn] HΦ").
+    by iFrame "#".
+  - wp_cmpxchg_fail.
+    iFrame; iModIntro; wp_pures.
+    by iApply "IH".
+Qed.
 
 Lemma release_spec γ l P :
   {{{ is_lock γ l P ∗ locked γ ∗ P }}} release l {{{ RET #(); True }}}.
 Proof.
-  (* exercise *)
-Admitted.
+  iIntros "%Φ ((%lo & %ln & -> & #I) & [%o Hγ] & P) HΦ".
+  wp_lam; wp_pures.
+  wp_bind (! _)%E.
+  iInv "I" as "(%o' & %n & Hlo & Hln & Hγ' & [[>Ho' _] | Ho])".
+  { iCombine "Hγ Ho'" gives "%H".
+    rewrite auth_frag_valid pair_valid /= in H.
+    by destruct H. }
+  wp_load.
+  iCombine "Hγ Hγ'" gives "%H".
+  rewrite cmra_comm auth_both_valid_discrete pair_included Excl_included in H.
+  assert (o ≡ o') as [] by intuition.
+  iModIntro.
+  iFrame "Hlo Hln Hγ' Ho".
+  wp_pures; clear.
+  rewrite Z.add_comm -(Nat2Z.inj_add 1) /=.
+  iInv "I" as "(%o' & %n & Hlo & Hln & Hγ' & [[>Ho' _]|Ho])".
+  { iCombine "Hγ Ho'" gives "%H".
+    rewrite auth_frag_valid pair_valid /= in H.
+    by destruct H. }
+  wp_store.
+  iAssert (True)%I as "⊤"; first done.
+  iPoseProof ("HΦ" with "⊤") as "HΦ"; iClear "⊤".
+  iCombine "Hγ Hγ'" gives "%H".
+  rewrite cmra_comm auth_both_valid_discrete pair_included Excl_included in H.
+  assert (o ≡ o') as [] by intuition.
+  iFrame "Hlo ∗"; clear.
+  iCombine "Hγ Hγ'" as "Hγ".
+  iMod (own_update _ _ (● (Excl' (S o), GSet (set_seq 0 n)) ⋅ ◯ (Excl' (S o), GSet ∅)) with "Hγ") as "[Hγ Ho']".
+  { rewrite cmra_comm.
+    by apply auth_update, prod_local_update_1, 
+             option_local_update, exclusive_local_update. }
+  iCombine "Ho' P" as "HP".
+  by iFrame. 
+Qed.
 
 End proofs.
